\documentclass[UTF8]{ctexart}
\usepackage{amsmath}
\title{第一周作业}
\author{邓贤杰}
\date{\today}

\begin{document}
    \maketitle
    \paragraph*{3}
    \begin{align*}
        &\iint \limits_D ydxdy \\
        = &\int_0^{\pi}dx\int_0^{sinx}ydy \\
        = &\int_0^{\pi}\frac{sin^2 x}{2}dx \\
        = &(\frac{x}{4}-\frac{sin2x}{8}) \big|_0^{\pi} \\
        = &\frac{\pi}{4}
    \end{align*}
    \paragraph*{4}
    \begin{align*}
        &\iint \limits_D xy^2dxdy \\
        =&\int_{-2}^{2}dy \int_{\frac{y^2}{4}}^{1} xy^2 dx \\
        =&\int_{-2}^{2} \frac{y^2}{2}-\frac{y^6}{32}dy\\
        =&\frac{32}{21}
    \end{align*}
\paragraph{5}
    \begin{align*}
        &\iint \limits_D e^{\frac{x}{y}}dxdy \\
        =&\int_0^1 dy \int_{0}^{y^2} e^{\frac{x}{y}}dx \\
        =&\int_{0}^{1} (ye^y - y)dy \\
        =& ye^y \big|_0^1 - \int_{0}^{1} e^y dy - \frac{y^2}{2} \big|_0^1\\
        =& \frac{1}{2}  
    \end{align*}
\paragraph*{6}
    \begin{align*}
        &\int_{0}^{1} dy \int_{y^{\frac{1}{3}}}^{1}\sqrt{1-x^4} dx \\
        =& \int_{0}^{1} dx \int_{0}^{x^3} \sqrt{1-x^4} dy \\
        =& -\frac{1}{4} \int_{0}^{1} \sqrt{1-x^4} \mathrm{d}(1-x^4) \\
        =& -\frac{1}{6} (1-x^4)^{\frac{3}{2}} \big|_{0}^{1} \\
        =& \frac{1}{6} 
    \end{align*}
\paragraph*{8}
\begin{align*}
    &\int_{0}^{\pi} \mathrm{d}x \int_{x}^{\pi} \frac{siny}{y} \mathrm{d}y \\
    = &\int_{0}^{\pi} \mathrm{d}y \int_{0}^{y} \frac{siny}{y} \mathrm{d}x \\
    = &\int_{0}^{\pi} siny \mathrm{d}y \\
    = &2
\end{align*}
\paragraph*{9}
\begin{align*}
    &\int_{0}^{2} \mathrm{d}x \int_{x}^{2} 2y^2sin(xy)\mathrm{d}y \\
    = &\int_{0}^{2} \mathrm{d}y \int_{0}^{y} 2y^2sin(xy)\mathrm{d}x \\
    =& \int_{0}^{2} \mathrm{d}y (-\frac{cos(xy)}{y} \big|_{0}^{y}) \\
    =& \int_{0}^{2} (1-cos(y^2))\mathrm{d}(y^2) \\
    =&4-sin4
\end{align*}
\paragraph*{10}
\begin{align*}
    & \iint \limits_D y^2 \sqrt{1-x^2} \mathrm{d}\sigma \\
    =& \int_{-1}^{1} \mathrm{d}x \int_{\sqrt{1-x^2}}^{-\sqrt{1-x^2} } y^2 \sqrt{1-x^2} \mathrm{d}y \\
    =&  \frac{2}{3} \int_{-1}^{1}  (1-x^2)^2 \mathrm{d}x \\
    =& \frac{32}{45} 
\end{align*}
\paragraph*{11}
按照$x$的正负将$D$划分为$D_1$和$D_2$
\begin{align*}
    & \iint \limits_D (|x| + y) \mathrm{d}\sigma \\
    =& \iint \limits_{D_1} (x+y) \mathrm{d}\sigma + \iint \limits_{D_2} (y-x) \mathrm{d}\sigma \\
    & \iint \limits_{D_1} (x+y) \mathrm{d}\sigma \\
    =& \int_{0}^{1} \mathrm{d}x\int_{x-1}^{1-x} (x+y)\mathrm{d}y \\
    =& \int_{0}^{1} 2x(1-x)\mathrm{d}x \\
    =& \frac{1}{3}  \\
    & \iint \limits_{D_2} (y-x) \mathrm{d}\sigma \\
    =& \int_{-1}^{0} \mathrm{d}x \int_{-x-1}^{x+1} (y-x)\mathrm{d}y \\
    =& \int_{-1}^{0} -2x(x+1)\mathrm{d}x \\
    =& \frac{1}{3} 
\end{align*}
故所求为$\frac{2}{3}$
\paragraph*{13}
\begin{align*}
    \int_{0}^{1} \mathrm{d}x \int_{\sqrt{1-x^2} }^{0} (x^2 + y^2)\mathrm{d}y 
\end{align*}
\paragraph*{15}
\begin{align*}
    \int_{0}^{2} \mathrm{d}x \int_{0}^{\sqrt{1-(x-1)^2}}3xy \mathrm{d}y 
\end{align*}
\paragraph*{18}
\begin{align*}
    \iint \limits_D r \mathrm{d}\sigma
\end{align*}
\paragraph*{19}
证：
\begin{align*}
    S=& \iint \limits_D \mathrm{d}x \mathrm{d}y \\
     =& \iint \limits_D r \mathrm{d}r \mathrm{d}\theta \\
     =& \int_{\alpha}^{\beta} \int_{0}^{r(\theta)} r \mathrm{d}r \\
     =& \frac{1}{2} \int_{\alpha}^{\beta} [r(\theta)]^2 \mathrm{d}\theta
\end{align*}
\paragraph*{20}
设所求面积为$S$
\begin{align*}
    \frac{1}{2}S=& \iint \limits_D \mathrm{d}x \mathrm{d}y \\
     =& \iint \limits_D rd \mathrm{d}r \mathrm{d}\theta \\
     =& \int_{0}^{\pi} \mathrm{d}\theta \int_{0}^{a(1 + cos\theta)} r \mathrm{d}r
\end{align*}
\end{document}