\documentclass[UTF8]{ctexart}
\usepackage{amsmath}
\title{第三周作业}
\author{邓贤杰}
\date{\today}

\begin{document}
    \maketitle
    \paragraph*{P60.4}
    \begin{align*}
        &\int_{L}^{} \frac{1}{x^2+y^2+z^2} \mathrm{d}s \\
        =& \int_{0}^{2\pi} \frac{1}{a^2 cos^2t + a^2 sin^2t +b^2t^2} \sqrt{a^2sin^2+a^2cos^2+b^2} \mathrm{d}t \\
        =& \int_{0}^{2\pi} \frac{1}{a^2+b^2t^2} \sqrt{a^2+b^2} \mathrm{d}t \\ 
        =& \frac{\sqrt{a^2+b^2}}{ab} \int_{0}^{2\pi} \frac{1}{1+\frac{b^2t^2}{a^2} }\mathrm{d}\left(\frac{bt}{a}\right) \\
        =& \frac{\sqrt{a^2+b^2}}{ab} \arctan \frac{bt}{a} \big|_{0}^{2\pi} \\
        =& \frac{\sqrt{a^2+b^2}}{ab} \arctan \frac{2b\pi}{a}
    \end{align*}
    \paragraph*{P60.6}

    令
    \begin{equation}
     \begin{cases}
         x = acos\theta \\
        y = bsin\theta \\
     \end{cases}
    \end{equation}

    则
    \begin{align*}
        \mathrm{d}s =& \sqrt{a^2 \sin^2 \theta+b^2 \cos ^2 \theta} \mathrm{d}\theta \\
        =& \sqrt{\frac{a^2+b^2}{2} + \frac{a^2-b^2}{2} \cos 2\theta} \mathrm{d}\theta\\
    \end{align*}

    故
    \begin{align*}
        &\int_{L}^{} xy \mathrm{d}s \\
        =& \int_{L}^{} ab \sin \theta \cos \theta \mathrm{d}s \\
        =& \int_{L}^{} \frac{1}{2} ab \sin 2\theta \mathrm{d}s \\
        =&-\int_{0}^{\frac{\pi}{2} } \frac{1}{2} ab \sin 2\theta
        \sqrt{\frac{a^2+b^2}{2} + \frac{a^2-b^2}{2} \cos 2\theta} \mathrm{d}\theta \\
        =&-\int_{0}^{\frac{\pi}{2} }
        \frac{1}{4} ab 
        \sqrt{\frac{a^2+b^2}{2} + \frac{a^2-b^2}{2} \cos 2\theta} 
        \mathrm{d}(\cos 2\theta) \\
        =& -\frac{ab}{3(a^2 - b ^2)} \left(\frac{a^2+b^2}{2} + \frac{a^2-b^2}{2} \cos 2\theta \right) \mathrm{d}\theta 
        \big|_{0}^{\frac{\pi}{2} } \\
        =& \frac{ab(a^3-b^3)}{3(a^2-b^2)} \\
        =& \frac{ab(a^2+ab+b^2)}{3(a+b)} 
    \end{align*}

    \paragraph*{P60.7}

    由
    \begin{align*}
        ds =& \sqrt{x'(t)^2 + y'(t)^2} dt \\
        =& |a|t \mathrm{d}t  
    \end{align*}

    有
    \begin{align*}
        &\int_{L} \sqrt{x^2+y^2} \mathrm{d}s \\
        =& \int_{0}^{2\pi} a^2\sqrt{1+t^2}t \mathrm{d}t \\
        =& \int_{0}^{2\pi} \frac{a^2}{2} \sqrt{1+t^2} \mathrm{d}(1+t^2) \\
        =& \frac{a^2}{3} (1+4\pi^2)^{\frac{3}{2} } - \frac{a^2}{3} 
    \end{align*}
    \paragraph*{P60.8}
    \begin{align*}
        &\int_{L} (x+\sqrt{y} -z^5)\mathrm{d}s \\
        =& \int_{L1}^{} 2x \mathrm{d}s + \int_{L2}^{} 2-z^5 \mathrm{d}s \\
    \end{align*}

    其中
    \begin{align*}
        &\int_{L1}^{} 2x \mathrm{d}s \\
        =& \int_{0}^{1} 2x \sqrt{1+(2x)^2} \mathrm{d}x \\
        =& \frac{1}{4} \int_{0}^{1} \sqrt{4x^2+1} \mathrm{d}(x^2) \\
        =& \frac{1}{6} (4x^2+1)^{\frac{3}{2} } \big|_{0}^{1} \\
        =& \frac{5\sqrt{5}-1}{6} 
    \end{align*}
    \begin{align*}
        &\int_{L2}^{} 2-z^5 \mathrm{d}s \\
        =& \int_{0}^{1} (2-z^5)\mathrm{d}z \\
        =& (2z-\frac{z^6}{6} )\big|_{0}^{1} \\
        =&\frac{11}{6} 
    \end{align*}

    所以所求为\[
        \frac{5\sqrt{5}+10}{6} 
    \]
    \paragraph*{P70.1}
    \subparagraph*{(1)}

    有
    \begin{align*}
        L:y=\frac{x}{2} 
    \end{align*}

    故
    \begin{align*}
        &\int_{L} 2xy \mathrm{d}x - x^2 \mathrm{d}y \\
        =& \int_{0}^{2} \frac{x^2}{2} \mathrm{d}x \\
        =& \frac{4}{3} 
    \end{align*}
    \subparagraph*{(2)}
    有
    \begin{align*}
        L:y=\frac{x^2}{4} 
    \end{align*}

    故
    \begin{align*}
        &\int_{L} 2xy \mathrm{d}x - x^2 \mathrm{d}y \\
        =& \int_{0}^{2} (2x\cdot \frac{x^2}{4} \mathrm{d}x - x^2 \cdot \frac{x}{2} \mathrm{d}x) \\
        = 0
    \end{align*}
    \subparagraph*{(3)}
    有
    \begin{equation*}
        \begin{cases}
            L_1:y=0\\
            L_2:x=2\\
        \end{cases}
    \end{equation*}

    故
    \begin{align*}
        &\int_{L} 2xy \mathrm{d}x - x^2 \mathrm{d}y \\
        =& \int_{L1} 2xy \mathrm{d}x - x^2 \mathrm{d}y + \int_{L2} 2xy \mathrm{d}x - x^2 \mathrm{d}y \\
        =& \int_{0}^{1} -4y \mathrm{d}y \\
        =& -4
    \end{align*}

    \subparagraph*{(4)}
    有
    \begin{equation}
        \begin{cases}
            L_1:x=0 \\
            L_2:y=1 \\
        \end{cases}
    \end{equation}

    故
    \begin{align*}
        &\int_{L} 2xy \mathrm{d}x - x^2 \mathrm{d}y \\
        =& \int_{L1} 2xy \mathrm{d}x - x^2 \mathrm{d}y + \int_{L2} 2xy \mathrm{d}x - x^2 \mathrm{d}y \\
        =&\int_{0}^{2} 2x \mathrm{d}x \\
        =& 4
    \end{align*}
    \paragraph*{P71.4}
    \subparagraph*{(1)}
    
    \begin{align*}
        &\int_{L}^{} (x^2-2xy) \mathrm{d}x + (y^2-2xy) \mathrm{d}y \\
        =& \int_{-1}^{1} x^2-2x^5+4x^{11}-8x^8 \\
        =& -\frac{10}{9} 
    \end{align*}

    \subparagraph*{(2)}
    \begin{align*}
        &\int_{L}^{} (x^2-2xy) \mathrm{d}x + (y^2-2xy) \mathrm{d}y \\
        =& \int_{-1}^{1} (x^2-2x) \mathrm{d}x \\
        =& \frac{2}{3} 
    \end{align*}
\paragraph*{P71.5}
\begin{align*}
    &\oint_{L} y \mathrm{d}x + z \mathrm{d}y + x \mathrm{d}z \\
    =& \int_{0}^{2\pi} (-a^2\sin^2t + abt\cos t + ab\cos t) \mathrm{d}t \\
    & \int_{0}^{2\pi} -a^2sin^2t \mathrm{d}t \\
    =& \frac{a^2}{4} (sin2t - 2t)\big|_{0}^{2\pi} = -a^2\pi  \\
    & \int_{0}^{2\pi} abtcost  \mathrm{d}t \\
    =& abt\sin t \big|_{0}^{2\pi}  - ab \int_{0}^{2\pi} sint \mathrm{d}t \\
    =& ab\cos t \big|_{0}^{2\pi} \\
    =& 0 \\
     & \int_{0}^{2\pi}abcost \mathrm{d}t \\
    =& absint \big|_{0}^{2\pi} = 0
\end{align*}

故所求为$-\pi a^2$
\paragraph*{P71.6}
令
\begin{equation*}
    \begin{cases}
        L_1: y=-x ,x \in [-1, 0] \\
        L_2: y=x, x \in (0, 2]
    \end{cases}
\end{equation*}

故
\begin{align*}
  &\int_{L}^{} (x^2+y^2) \mathrm{d}x + (x^2 - y) \mathrm{d}y \\
  =& \int_{L_1}^{} (x^2+y^2) \mathrm{d}x + (x^2 - y) \mathrm{d}y + 
  \int_{L_2}^{} (x^2+y^2) \mathrm{d}x + (x^2 - y) \mathrm{d}y \\
  =& \int_{-1}^{0} (x^2-x) \mathrm{d}x + \int_{0}^{2} (3x^3 - x)\mathrm{d}x \\
  =& \frac{41}{6} 
\end{align*}
\paragraph*{P71.8}
\begin{align*}
    &\int_{L}^{} (x^4-z^2)\mathrm{d}x+2xy^2 \mathrm{d}y - y \mathrm{d}z \\
    =& \int_{0}^{1} ((t^4-t^6)\mathrm{d}t + 4t^6 \mathrm{d}t - 3t^4 \mathrm{d}t) \\
    =& \int_{0}^{1} (-2t^4+3t^6) \mathrm{d}t \\
    =& \frac{1}{35} 
\end{align*}
\paragraph*{P88.2(2)}
\begin{align*}
    S =& \frac{1}{2} \oint_{L_+} x \mathrm{d}y -y \mathrm{d}x \\
    =& \frac{a^2}{2} \int_{0}^{2\pi} (1-\cos t) \sin t [\sin t \cos t -(1-\cos t)\sin t] \\
    =& \frac{a^2}{2} \int_{0}^{2\pi} (1-\cos t) ^ 2 \mathrm{d}t \\
    =& \frac{a^2}{2}\left(\frac{\sin 2t}{4} - 2 \sin t + \frac{3}{2} t \right) \big|_{0}^{2\pi}\\
    =& \frac{3}{2} \pi a^2
\end{align*}
\paragraph*{P88.4}
\subparagraph*{(1)}
\begin{align*}
    &(x+y)\mathrm{d}x+(x-y)\mathrm{d}y \\
    =& \mathrm{d}(xy + \frac{x^2-y^2}{2} + c) \\
    =& \mathrm{d}u
\end{align*}

故路径无关，且
\begin{align*}
    &\int_{(0,0)}^{(1,1)} (x+y)\mathrm{d}x+(x-y)\mathrm{d}y \\
    =& u(1,1) - u(0, 0) = 1 - 0 = 0
\end{align*}
\subparagraph*{(3)}
\begin{align*}
    &e^x\cos y \mathrm{d}x - e^x \sin y \mathrm{d}y \\
    =& \mathrm{d}(e^x \cos y) = \mathrm{d}u
\end{align*}

故与路径无关，且
\begin{align*}
    &\int_{(0,0)}^{(a,b)} e^x \cos y \mathrm{d}x - e^x \sin y \mathrm{d}y \\
    =& u(a,b) - u(0, 0) = e^a \cos b - 1
\end{align*}
\paragraph*{P88.9}
\begin{align*}
    & (x^2+y)\mathrm{d}x + (x - y^2) \mathrm{d}y \\
    =& \mathrm{d}\left(xy+\frac{x^3 -y ^3}{3} \right) = \mathrm{d}u
\end{align*}

故
\begin{align*}
    &\int_{\overset{\frown}{AB}}^{} (x^2+y)\mathrm{d}x + (x - y^2) \mathrm{d}y \\
    =& u(1,1) - u(0, 0) = 1 - 0 = 1
\end{align*}
\end{document}